Updated the rest of the files to coincide with cat2funcset version.

HybridVerifVecs/nd_funs/cat2ndfun.thy
@@ -3,8 +3,7 @@ theory cat2ndfun
                         
 begin
 
-
-section{* Hybrid System Verification *}
+section{* Hybrid System Verification with nondeterministic functions *}
 
 \<comment> \<open>We start by deleting some conflicting notation and introducing some new.\<close>
 no_notation Archimedean_Field.ceiling ("\<lceil>_\<rceil>")
@@ -17,9 +16,15 @@ notation Abs_nd_fun ("_\<^sup>\<bullet>" [101] 100) and Rep_nd_fun ("_\<^sub>\<b
 
 subsection{* Nondeterministic Functions *}
 
-lemma Abs_nd_fun_inverse2[simp]:"(f\<^sup>\<bullet>)\<^sub>\<bullet> = f"
+text{* Our semantics correspond now to nondeterministic functions @{typ "'a nd_fun"}. Below we prove
+some auxiliary lemmas for them and show that they form an antidomain kleene algebra. The proof just 
+extends the results on the Transformer\_Semantics.Kleisli\_Quantale theory.*}
+
+\<comment> \<open>Analog of already existing @{thm Rep_nd_fun_inverse[no_vars]}.\<close>
+lemma Abs_nd_fun_inverse2[simp]:"(f\<^sup>\<bullet>)\<^sub>\<bullet> = f" 
   by(simp add: Abs_nd_fun_inverse)
 
+\<comment> \<open>Analog of already existing @{thm Rep_nd_fun_inverse[no_vars]}.\<close>
 lemma nd_fun_ext:"(\<And>x. (f\<^sub>\<bullet>) x = (g\<^sub>\<bullet>) x) \<Longrightarrow> f = g"
   apply(subgoal_tac "Rep_nd_fun f = Rep_nd_fun g")
   using Rep_nd_fun_inject apply blast
@@ -81,7 +86,9 @@ instance
   by(transfer; auto)+
 end
 
-subsection{* Weakest Liberal Preconditions *}
+text{* Now that we know that nondeterministic functions form an Antidomain Kleene Algebra, we give
+ a lifting operation from predicates to @{typ "'a nd_fun"} and prove some useful results for them. 
+Then we add an operation that does the opposite and prove the relationship between both of these. *}
 
 abbreviation p2ndf :: "'a pred \<Rightarrow> 'a nd_fun" ("(1\<lceil>_\<rceil>)")
   where "\<lceil>Q\<rceil> \<equiv> (\<lambda> x::'a. {s::'a. s = x \<and> Q s})\<^sup>\<bullet>"
@@ -114,7 +121,20 @@ lemma p2ndf_ndf2p_id:"F \<le> \<eta>\<^sup>\<bullet> \<Longrightarrow> \<lceil>\
   apply(subgoal_tac "\<forall>x. (F\<^sub>\<bullet>) x \<subseteq> {x}", simp)
   by(blast, simp add: le_fun_def less_eq_nd_fun.rep_eq)
 
+lemma ndf2p_p2ndf_id:"\<lfloor>\<lceil>P\<rceil>\<rfloor> = P"
+  by(simp add: f2r_def)
+
+subsection{* Verification of regular programs *}
+
+text{* As expected, the weakest precondition is just the forward box operator from the KAD. Below 
+we explore its behavior with the previously defined lifting ($\lceil-\rceil$*) and dropping ($\lfloor-\rfloor$*)
+operators *}
+
 abbreviation "wp f \<equiv> fbox (f::'a nd_fun)"
+
+lemma wp_eta[simp]:"wp (\<eta>\<^sup>\<bullet>) \<lceil>P\<rceil> = \<lceil>P\<rceil>"
+  apply(simp add: fbox_def, transfer, simp)
+  by(rule nd_fun_ext, auto simp: kcomp_def)
 
 lemma wp_nd_fun:"wp (F\<^sup>\<bullet>) \<lceil>P\<rceil> = \<lceil>\<lambda> x. \<forall> y. y \<in> (F x) \<longrightarrow> P y\<rceil>"
   apply(simp add: fbox_def, transfer, simp)
@@ -142,29 +162,22 @@ lemma p2ndf_ndf2p_wp:"\<lceil>\<lfloor>wp R P\<rfloor>\<rceil> = wp R P"
 lemma p2ndf_ndf2p_wp_sym:"wp R P = \<lceil>\<lfloor>wp R P\<rfloor>\<rceil>"
   by(rule sym, simp add: p2ndf_ndf2p_wp)
 
-lemma wp_trafo: "\<lfloor>wp F \<lceil>Q\<rceil>\<rfloor> s = (\<forall>s'. s' \<in> (F\<^sub>\<bullet>) s \<longrightarrow> Q s')"  
+lemma ndf2p_wpD: "\<lfloor>wp F \<lceil>Q\<rceil>\<rfloor> s = (\<forall>s'. s' \<in> (F\<^sub>\<bullet>) s \<longrightarrow> Q s')"  
   apply(subgoal_tac "F = (F\<^sub>\<bullet>)\<^sup>\<bullet>")
   apply(rule ssubst[of F "(F\<^sub>\<bullet>)\<^sup>\<bullet>"], simp)
   apply(subst wp_nd_fun)
   by(simp_all add: f2r_def)
 
-\<comment> \<open>Another characterization of the wp operator in terms of the forward box operator.\<close>
+text{* We can verify that our introduction of @{text "wp"} coincides with another definition of the 
+forward box operator @{thm ffb_def[no_vars]} with the following characterization lemmas. *}
+
 lemma ffb_is_wp:"fb\<^sub>\<F> (F\<^sub>\<bullet>) {x. P x} = {s. \<lfloor>wp F \<lceil>P\<rceil>\<rfloor> s}"
   unfolding ffb_def unfolding map_dual_def klift_def kop_def fbox_def
   unfolding r2f_def f2r_def apply clarsimp
   unfolding antidomain_op_nd_fun_def unfolding dual_set_def 
   unfolding times_nd_fun_def kcomp_def by force
 
-lemma wp_is_ffb:"wp F \<lceil>P\<rceil> = (\<lambda>x. {x} \<inter> fb\<^sub>\<F> (F\<^sub>\<bullet>) {s. P s})\<^sup>\<bullet>"
-  apply(rule nd_fun_ext, simp)
-  apply(subgoal_tac "F = (F\<^sub>\<bullet>)\<^sup>\<bullet>")
-   apply(rule ssubst[of F "(F\<^sub>\<bullet>)\<^sup>\<bullet>"], simp)
-  apply(subst wp_nd_fun)
-   apply(subst ffb_is_wp)
-   apply(subst wp_trafo)
-  by auto
-
-lemma wp_is_ffb2:"wp F P = (\<lambda>x. {x} \<inter> fb\<^sub>\<F> (F\<^sub>\<bullet>) {s. \<lfloor>P\<rfloor> s})\<^sup>\<bullet>"
+lemma wp_is_ffb:"wp F P = (\<lambda>x. {x} \<inter> fb\<^sub>\<F> (F\<^sub>\<bullet>) {s. \<lfloor>P\<rfloor> s})\<^sup>\<bullet>"
   apply(rule nd_fun_ext, simp)
   unfolding ffb_def unfolding map_dual_def klift_def kop_def fbox_def
   unfolding r2f_def f2r_def apply clarsimp
@@ -173,6 +186,7 @@ lemma wp_is_ffb2:"wp F P = (\<lambda>x. {x} \<inter> fb\<^sub>\<F> (F\<^sub>\<bu
   unfolding kcomp_prop apply auto
   by (metis (full_types, lifting) Int_Collect UnCI empty_not_insert ex_in_conv image_eqI)
 
+text{* Next, we introduce assignments and compute their @{text "wp"}. *}
 
 abbreviation vec_upd :: "('a^'b) \<Rightarrow> 'b \<Rightarrow> 'a \<Rightarrow> 'a^'b" ("_(2[_ :== _])" [70, 65] 61) where 
 "x[i :== a] \<equiv> (\<chi> j. (if j = i then a else (x $ j)))"
@@ -183,6 +197,11 @@ abbreviation assign :: "'b \<Rightarrow> ('a^'b \<Rightarrow> 'a) \<Rightarrow> 
 lemma wp_assign[simp]: "wp ([x ::== expr]) \<lceil>Q\<rceil> = \<lceil>\<lambda>s. Q (s[x :== expr s])\<rceil>"
   by(subst wp_nd_fun, rule nd_fun_ext, simp)
 
+text{* The @{text "wp"} of the composition was already obtained in KAD.Antidomain\_Semiring:
+@{thm fbox_mult[no_vars]}. *}
+
+text{* We also have an implementation of the conditional operator and its @{text "wp"}. *}
+
 definition (in antidomain_kleene_algebra) cond :: "'a \<Rightarrow> 'a \<Rightarrow> 'a \<Rightarrow> 'a" 
 ("if _ then _ else _ fi" [64,64,64] 63) where "if p then x else y fi = d p \<cdot> x + ad p \<cdot> y"
 
@@ -190,7 +209,7 @@ abbreviation cond_sugar :: "'a pred \<Rightarrow> 'a nd_fun \<Rightarrow> 'a nd_
 ("IF _ THEN _ ELSE _ FI" [64,64,64] 63) where
   "IF P THEN X ELSE Y FI \<equiv> cond \<lceil>P\<rceil> X Y"
 
-lemma ffb_if_then_else:
+lemma wp_if_then_else:
   assumes "\<lceil>\<lambda>s. P s \<and> T s\<rceil> \<le> wp X \<lceil>Q\<rceil>"
     and "\<lceil>\<lambda>s. P s \<and> \<not> T s\<rceil> \<le> wp Y \<lceil>Q\<rceil>"
   shows "\<lceil>P\<rceil> \<le> wp (IF T THEN X ELSE Y FI) \<lceil>Q\<rceil>"
@@ -198,6 +217,8 @@ lemma ffb_if_then_else:
   apply(subst (asm) wp_nd_fun2)+
   unfolding cond_def apply(clarsimp, transfer)
   by(auto simp: kcomp_prop)
+
+text{* Finally we also deal with finite iteration. *}
 
 lemma (in antidomain_kleene_algebra) fbox_starI: 
 assumes "d p \<le> d i" and "d i \<le> |x] i" and "d i \<le> d q"
@@ -234,16 +255,6 @@ proof-
     using \<open>d P = P\<close> by (transfer, simp)
 qed
 
-lemma ffb_starI:
-assumes "{x. P x} \<le> {x. I x}" and "{x. I x} \<le> fb\<^sub>\<F> (F\<^sub>\<bullet>) {x. I x}" and "{x. I x} \<le> {x. Q x}"
-shows "{x. P x} \<le> fb\<^sub>\<F> ((qstar F)\<^sub>\<bullet>) {x. Q x}"
-proof-
-  from assms(1,3) have "\<lceil>P\<rceil> \<le> \<lceil>I\<rceil> \<and> \<lceil>I\<rceil> \<le> \<lceil>Q\<rceil>" by auto
-  also from assms(2) have "\<lceil>I\<rceil> \<le> wp F \<lceil>I\<rceil>" by(subst wp_is_ffb, transfer, auto simp: le_fun_def)
-  ultimately have "\<lceil>P\<rceil> \<le> wp (qstar F) \<lceil>Q\<rceil>" using wp_starI by blast
-  from this show ?thesis by(subst (asm) wp_is_ffb, transfer, auto simp: le_fun_def)
-qed
-
 subsection{* Verification by providing solutions *}
 
 abbreviation "orbital f T S t0 x0 \<equiv> 
@@ -259,7 +270,7 @@ context picard_ivp
 begin
 
 lemma orbital_collapses: 
-  assumes ivp:"\<forall>s \<in> S. ((\<lambda>t. \<phi> t s) solves_ode f)T S \<and> \<phi> t0 s = s" and "s \<in> S"
+  assumes "\<forall>s \<in> S. ((\<lambda>t. \<phi> t s) solves_ode f)T S \<and> \<phi> t0 s = s" and "s \<in> S"
   shows "orbital f T S t0 s = {\<phi> t s| t. t \<in> T}"
   apply safe apply(rule_tac x="t" in exI, simp)
    apply(rule_tac x="xa" and s="xa t0" in unique_solution, simp_all add: assms)
@@ -267,7 +278,7 @@ lemma orbital_collapses:
   using assms init_time by auto
 
 lemma g_orbital_collapses: 
-  assumes ivp:"\<forall>s \<in> S. ((\<lambda>t. \<phi> t s) solves_ode f)T S \<and> \<phi> t0 s = s" and "s \<in> S"
+  assumes "\<forall>s \<in> S. ((\<lambda>t. \<phi> t s) solves_ode f)T S \<and> \<phi> t0 s = s" and "s \<in> S"
   shows "g_orbital f T S t0 s G = {\<phi> t s| t. t \<in> T \<and> (\<forall> r \<in> {t0--t}. G (\<phi> r s))}"
   apply safe apply(rule_tac x="t" in exI, simp) 
   using assms unique_solution apply(metis closed_segment_subset_domainI)
@@ -275,23 +286,23 @@ lemma g_orbital_collapses:
   using assms init_time by auto
 
 lemma wp_orbit:
-  assumes ivp:"\<forall>s \<in> S. ((\<lambda>t. \<phi> t s) solves_ode f)T S \<and> \<phi> t0 s = s"
+  assumes "\<forall>s \<in> S. ((\<lambda>t. \<phi> t s) solves_ode f)T S \<and> \<phi> t0 s = s"
   shows "wp ((\<lambda> s. orbital f T S t0 s)\<^sup>\<bullet>) \<lceil>Q\<rceil> = \<lceil>\<lambda> s. \<forall> t \<in> T. s \<in> S \<longrightarrow> Q (\<phi> t s)\<rceil>"
   apply(subst wp_nd_fun, subst eq_p2ndf_iff) apply(rule ext, safe)
    apply(erule_tac x="\<phi> t s" in allE, erule impE, simp)
     apply(rule_tac x="t" in exI, rule_tac x="\<lambda> t. \<phi> t s" in exI)
-  using ivp init_time apply(simp, simp)
+  using assms init_time apply(simp, simp)
   apply(subgoal_tac "\<phi> t (x t0) = x t")
    apply(erule_tac x="t" in ballE, simp, simp)
   by(rule_tac y="x" and s="x t0" in unique_solution, simp_all add: assms)
 
 lemma wp_g_orbit:
-  assumes ivp:"\<forall>s \<in> S. ((\<lambda>t. \<phi> t s) solves_ode f)T S \<and> \<phi> t0 s = s"
-  shows "wp {[x\<acute>=f]T S @ t0 & G} \<lceil>Q\<rceil> = \<lceil>\<lambda> s. \<forall> t \<in> T. s \<in> S \<longrightarrow> (\<forall> r \<in> {t0--t}.G (\<phi> r s)) \<longrightarrow> Q (\<phi> t s)\<rceil>"
+  assumes "\<forall>s \<in> S. ((\<lambda>t. \<phi> t s) solves_ode f)T S \<and> \<phi> t0 s = s"
+  shows "wp {[x\<acute>=f]T S @ t0 & G} \<lceil>Q\<rceil> = \<lceil>\<lambda> s. \<forall>t\<in>T. s\<in>S \<longrightarrow> (\<forall> r\<in>{t0--t}.G (\<phi> r s)) \<longrightarrow> Q (\<phi> t s)\<rceil>"
   apply(subst wp_nd_fun, subst eq_p2ndf_iff) apply(rule ext, safe)
    apply(erule_tac x="\<phi> t s" in allE, erule impE, simp)
     apply(rule_tac x="t" in exI, rule_tac x="\<lambda> t. \<phi> t s" in exI)
-  apply(simp add: ivp init_time, simp)
+  apply(simp add: assms init_time, simp)
   apply(subgoal_tac "\<forall>r\<in>{t0--t}. \<phi> r (x t0) = x r")
    apply(erule_tac x="t" in ballE, safe)
     apply(erule_tac x="r" in ballE)+ apply simp_all
@@ -301,6 +312,9 @@ lemma wp_g_orbit:
 
 end
 
+text{* The previous theorem allows us to compute wlps for known systems of ODEs. We can also implement
+a version of it as an inference rule. A simple computation of a wlp is shown immmediately after.*}
+
 lemma dSolution:
   assumes "picard_ivp f T S L t0" and ivp:"\<forall>s \<in> S. ((\<lambda>t. \<phi> t s) solves_ode f)T S \<and> \<phi> t0 s = s"
     and "\<forall>s. P s \<longrightarrow> (\<forall> t \<in> T. s \<in> S \<longrightarrow> (\<forall> r \<in> {t0..t}.G (\<phi> r s)) \<longrightarrow> Q (\<phi> t s))"
@@ -308,7 +322,6 @@ lemma dSolution:
   using assms apply(subst picard_ivp.wp_g_orbit, auto)
   by (simp add: Starlike.closed_segment_eq_real_ivl)
 
-text{* This last theorem allows us to compute weakest liberal preconditions for known systems of ODEs: *}
 corollary line_DS: "0 \<le> t \<Longrightarrow> wp {[x\<acute>=\<lambda>t s. c]{0..t} UNIV @ 0 & G} \<lceil>Q\<rceil> = 
     \<lceil>\<lambda> x. \<forall> \<tau> \<in> {0..t}. (\<forall>r\<in>{0--\<tau>}. G (x + r *\<^sub>R c)) \<longrightarrow> Q (x + \<tau> *\<^sub>R c)\<rceil>"
   apply(subst picard_ivp.wp_g_orbit[of "\<lambda> t s. c" _ _ "1/(t + 1)" _ "(\<lambda> t x. x + t *\<^sub>R c)"])
@@ -376,348 +389,121 @@ next show "\<And> a. g_orbital f T S t0 a (\<lambda> s. G s \<and> C s) \<subset
 qed
 
 theorem dCut:
-  assumes "t0 \<in> T" and "interval T"
-    and wp_C:"\<lceil>P\<rceil> \<le> wp ({[x\<acute>=f]T S @ t0 & G}) \<lceil>C\<rceil>"
-    and wp_Q:"\<lceil>P\<rceil> \<le> wp ({[x\<acute>=f]T S @ t0 & (\<lambda> s. G s \<and> C s)}) \<lceil>Q\<rceil>"
-  shows "\<lceil>P\<rceil> \<le> wp ({[x\<acute>=f]T S @ t0 & G}) \<lceil>Q\<rceil>"
+  assumes "t0 \<le> t" and wp_C:"\<lceil>P\<rceil> \<le> wp ({[x\<acute>=f]{t0..t} S @ t0 & G}) \<lceil>C\<rceil>"
+    and wp_Q:"\<lceil>P\<rceil> \<le> wp ({[x\<acute>=f]{t0..t} S @ t0 & (\<lambda> s. G s \<and> C s)}) \<lceil>Q\<rceil>"
+  shows "\<lceil>P\<rceil> \<le> wp ({[x\<acute>=f]{t0..t} S @ t0 & G}) \<lceil>Q\<rceil>"
 proof(subst wp_nd_fun, clarsimp)
-  fix t::real and x::"real \<Rightarrow> 'a" assume "P (x t0)" and "t \<in> T"  and "x t0 \<in> S"
-and x_solves:"(x solves_ode f)T S " and guard_x:"(\<forall> r \<in> {t0--t}. G (x r))"
-  from guard_x have "\<forall>r\<in>{t0--t}.\<forall> \<tau>\<in>{t0--r}. G (x \<tau>)"
-    using \<open>t0 \<in> T\<close> by (metis contra_subsetD ends_in_segment(1) subset_segment(1)) 
-  also have "\<forall>r\<in>{t0--t}. r \<in> T"
-    using \<open>t0 \<in> T\<close> \<open>interval T\<close> \<open>t \<in> T\<close> interval.closed_segment_subset_domain by blast
-  ultimately have "\<forall>r\<in>{t0--t}. x r \<in> g_orbital f T S t0 (x t0) G"
-    using x_solves \<open>x t0 \<in> S\<close> by blast
-  from this have "\<forall>r\<in>{t0--t}. C (x r)" using wp_C \<open>P (x t0)\<close> by(subst (asm) wp_nd_fun, simp)
-  hence "x t \<in> g_orbital f T S t0 (x t0) (\<lambda> s. G s \<and> C s)"
-    using guard_x  \<open>t \<in> T\<close>  x_solves \<open>x t0 \<in> S\<close> \<open>\<forall>r\<in>{t0--t}. r \<in> T\<close> by fastforce
-  from this \<open>P (x t0)\<close> and wp_Q show "Q (x t)"
-    by(subst (asm) wp_nd_fun, simp)
+  fix \<tau>::real and x::"real \<Rightarrow> 'a" assume "P (x t0)" and "t0 \<le> \<tau>" and "\<tau> \<le> t" and "x t0 \<in> S"
+    and x_solves:"(x solves_ode f){t0..t} S " and guard_x:"(\<forall> r \<in> {t0--\<tau>}. G (x r))"
+  hence "{t0--\<tau>} \<subseteq> {t0--t}" using closed_segment_eq_real_ivl by auto
+  from this and guard_x have "\<forall>r\<in>{t0--\<tau>}.\<forall>\<tau>\<in>{t0--r}. G (x \<tau>)"
+    using closed_segment_closed_segment_subset by blast
+  then have "\<forall>r\<in>{t0--\<tau>}. x r \<in> g_orbital f {t0..t} S t0 (x t0) G"
+    using x_solves \<open>x t0 \<in> S\<close> \<open>t0 \<le> \<tau>\<close> \<open>\<tau> \<le> t\<close> closed_segment_eq_real_ivl by fastforce
+  from this have "\<forall>r\<in>{t0--\<tau>}. C (x r)" using wp_C \<open>P (x t0)\<close> by(subst (asm) wp_nd_fun, auto)
+  hence "x \<tau> \<in> g_orbital f {t0..t} S t0 (x t0) (\<lambda> s. G s \<and> C s)"
+    using guard_x \<open>t0 \<le> \<tau>\<close> \<open>\<tau> \<le> t\<close> x_solves \<open>x t0 \<in> S\<close> by fastforce
+  from this \<open>P (x t0)\<close> and wp_Q show "Q (x \<tau>)"
+    by(subst (asm) wp_nd_fun, auto)
 qed
 
-corollary dCut_interval:
-  assumes "t0 \<le> t" and "\<lceil>P\<rceil> \<le> wp ({[x\<acute>=f]{t0..t} S @ t0 & G}) \<lceil>C\<rceil>" 
-    and "\<lceil>P\<rceil> \<le> wp ({[x\<acute>=f]{t0..t} S @ t0 & (\<lambda> s. G s \<and> C s)}) \<lceil>Q\<rceil>"
-  shows "\<lceil>P\<rceil> \<le> wp ({[x\<acute>=f]{t0..t} S @ t0 & G}) \<lceil>Q\<rceil>"
-  apply(rule_tac C="C" in dCut)
-  using assms by(simp_all add: interval_def)
-
-subsubsection{* Differential Invariant *}(* MODIFICATIONS REQUIRED: remove inf T*)
+subsubsection{* Differential Invariant *}
 
 lemma DI_sufficiency:
-  assumes "picard_ivp f T S L t0"
+  assumes "\<forall>s \<in> S. ((\<lambda>t. \<phi> t s) solves_ode f)T S \<and> \<phi> t0 s = s" and "t0 \<in> T"
   shows "wp {[x\<acute>=f]T S @ t0 & G} \<lceil>Q\<rceil> \<le> wp \<lceil>G\<rceil> \<lceil>\<lambda>s. s \<in> S \<longrightarrow> Q s\<rceil>"
   apply(subst wp_nd_fun, subst wp_nd_fun, clarsimp)
   apply(erule_tac x="s" in allE, erule impE, rule_tac x="t0" in exI, simp_all)
-  using assms picard_ivp.fixed_point_solves picard_ivp.init_time by metis
+  using assms by metis
 
-lemma 
-  fixes \<theta>::"'a::banach \<Rightarrow> real"
-  assumes "\<lceil>G\<rceil> \<le> \<lceil>I'\<rceil>" and "t \<ge> 0"
-    and "\<forall> x. (x solves_ode f){0..t} S \<longrightarrow> I (x 0) \<longrightarrow>
- (\<forall> t \<ge> 0. (\<forall>r\<in>{0--t}. I' (x r)) \<longrightarrow> (I (x t)))"
-  shows "\<lceil>I\<rceil> \<le> wp ({[x\<acute>=f]{0..t} S @ 0 & G}) \<lceil>I\<rceil>"
-  using assms apply(subst wp_nd_fun)
-  apply(subst le_p2ndf_iff) apply clarify
-  apply(erule_tac x="x" in allE)
-  apply(erule impE, simp)+
-  apply(erule_tac x="ta" in allE)
-  by simp
-
-definition pderivative :: "'a pred \<Rightarrow> 'a pred \<Rightarrow> (real \<Rightarrow> ('a::real_normed_vector) \<Rightarrow> 'a) \<Rightarrow> real set \<Rightarrow> 
-'a set \<Rightarrow> bool" ("(_)/ is'_pderivative'_of (_)/ with'_respect'_to (_) (_) (_)" [70, 65] 61) where
-"I' is_pderivative_of I with_respect_to f T S \<equiv> bdd_below T \<and> (\<forall> x. (x solves_ode f)T S \<longrightarrow> 
-I (x (Inf T)) \<longrightarrow> (\<forall> t \<in> T. (\<forall>r\<in>{(Inf T)--t}. I' (x r)) \<longrightarrow> (I (x t))))"
+definition ode_invariant :: "'a pred \<Rightarrow> (real \<Rightarrow> ('a::real_normed_vector) \<Rightarrow> 'a) \<Rightarrow> real set \<Rightarrow> 
+'a set \<Rightarrow> bool" ("(_)/ is'_ode'_invariant'_of (_) (_) (_)" [70,65]61) 
+  where "I is_ode_invariant_of f T S \<equiv> bdd_below T \<and> (\<forall> x. (x solves_ode f)T S \<longrightarrow>
+I (x (Inf T)) \<longrightarrow> (\<forall> t \<in> T. I (x t)))"
 
 lemma dInvariant:
-  assumes "\<lceil>G\<rceil> \<le> \<lceil>I'\<rceil>" and "I' is_pderivative_of I with_respect_to f T S"
-  shows "\<lceil>I\<rceil> \<le> wp ({[x\<acute>=f]T S @ (Inf T) & G}) \<lceil>I\<rceil>"
-  using assms unfolding pderivative_def apply(subst wp_nd_fun)
-  apply(subst le_p2ndf_iff)
-  by clarsimp
+  assumes "I is_ode_invariant_of f {t0..t} S"
+  shows "\<lceil>I\<rceil> \<le> wp ({[x\<acute>=f]{t0..t} S @ t0 & G}) \<lceil>I\<rceil>"
+  using assms unfolding ode_invariant_def apply(subst wp_nd_fun)
+  apply(subst le_p2ndf_iff, clarify)
+  apply(erule_tac x="x" in allE)
+  by(erule impE, simp_all)
 
 lemma dInvariant':
-  assumes "I' is_pderivative_of I with_respect_to f T S"
-    and "\<lceil>P\<rceil> \<le> \<lceil>I\<rceil>" and "\<lceil>G\<rceil> \<le> \<lceil>I'\<rceil>" and "\<lceil>I\<rceil> \<le> \<lceil>Q\<rceil>"
-  shows "\<lceil>P\<rceil> \<le> wp ({[x\<acute>=f]T S @ (Inf T) & G}) \<lceil>Q\<rceil>"
-  using assms unfolding pderivative_def apply(subst wp_nd_fun)
-  apply(subst le_p2ndf_iff)
-  by clarsimp
-
-lemma invariant_eq_0:
-  fixes \<theta>::"'a::banach \<Rightarrow> real"
-  assumes nuHyp:"\<forall> x. (x solves_ode f)T S \<longrightarrow> (\<forall> t \<in> T. \<forall> r \<in> {(Inf T)--t}. 
-  ((\<lambda>\<tau>. \<theta> (x \<tau>)) has_derivative (\<lambda>\<tau>. \<tau> *\<^sub>R \<nu> (x r))) (at r within {(Inf T)--t}))"
-    and "\<lceil>G\<rceil> \<le> \<lceil>\<lambda>s. \<nu> s = 0\<rceil>" and "bdd_below T"
-  shows "\<lceil>\<lambda>s. \<theta> s = 0\<rceil> \<le> wp ({[x\<acute>=f]T S @ (Inf T) & G}) \<lceil>\<lambda>s. \<theta> s = 0\<rceil>"
-  apply(rule dInvariant [of _ "\<lambda> s. \<nu> s = 0"])
-  using assms apply(simp, simp add: pderivative_def)
-proof(clarify)
-  fix x and t 
-  assume x_ivp:"(x solves_ode f) T S" "\<theta> (x (Inf T)) = 0"  
-    and tHyp:"t \<in> T" and eq0:"\<forall>r\<in>{Inf T--t}. \<nu> (x r) = 0"
-  hence "(Inf T) \<le> t" by (simp add: \<open>bdd_below T\<close> cInf_lower) 
-  have "\<forall> r \<in> {(Inf T)--t}. ((\<lambda>\<tau>. \<theta> (x \<tau>)) has_derivative (\<lambda>\<tau>. \<tau> *\<^sub>R \<nu> (x r))) 
-    (at r within {(Inf T)--t})" using nuHyp x_ivp(1) and tHyp by auto
-  then have "\<forall> r \<in> {(Inf T)--t}. ((\<lambda>\<tau>. \<theta> (x \<tau>)) has_derivative (\<lambda>\<tau>. \<tau> *\<^sub>R 0)) 
-    (at r within {(Inf T)--t})" using eq0 by auto
-  then have "\<exists>r\<in>{(Inf T)--t}. \<theta> (x t)- \<theta> (x (Inf T)) = (\<lambda>\<tau>. \<tau> *\<^sub>R 0) (t - (Inf T))" 
-    by(rule_tac closed_segment_mvt, auto simp: \<open>(Inf T) \<le> t\<close>)
-  thus "\<theta> (x t) = 0" 
-    using x_ivp(2) by (metis right_minus_eq scale_zero_right)
-qed
-
-corollary invariant_eq_0_interval:
-  fixes \<theta>::"'a::banach \<Rightarrow> real"
-  assumes "\<forall> x. (x solves_ode f){t0..t} S \<longrightarrow> (\<forall> \<tau> \<in> {t0..t}. \<forall> r \<in> {t0..\<tau>}. 
-  ((\<lambda>\<tau>. \<theta> (x \<tau>)) has_derivative (\<lambda>\<tau>. \<tau> *\<^sub>R (\<nu> (x r)))) (at r within {t0..\<tau>}))"
-    and "\<lceil>G\<rceil> \<le> \<lceil>\<lambda>s. \<nu> s = 0\<rceil>" and "t0 \<le> t"
-  shows "\<lceil>\<lambda>s. \<theta> s = 0\<rceil> \<le> wp ({[x\<acute>=f]{t0..t} S @ t0 & G}) \<lceil>\<lambda>s. \<theta> s = 0\<rceil>"
-  apply(subgoal_tac "\<lceil>\<lambda>s. \<theta> s = 0\<rceil> \<le> wp ({[x\<acute>=f]{t0..t} S @ (Inf {t0..t}) & G}) \<lceil>\<lambda>s. \<theta> s = 0\<rceil>")
-   apply(subgoal_tac "Inf {t0..t} = t0", simp)
-  using \<open>t0 \<le> t\<close> apply simp
-  apply(rule invariant_eq_0[of _ "{t0..t}" _ _ \<nu>])
-  using assms by(auto simp: closed_segment_eq_real_ivl)
-
-theorem dInvariant_eq_0:
-  fixes \<theta>::"'a::banach \<Rightarrow> real" and \<nu>::"'a \<Rightarrow> real"
-  assumes "\<forall>x. (x solves_ode f) {t0..t} S \<longrightarrow> 
-  (\<forall>\<tau>\<in>{t0..t}. \<forall>r\<in>{t0..\<tau>}. ((\<lambda>\<tau>. \<theta> (x \<tau>)) has_derivative (\<lambda>\<tau>. \<tau> *\<^sub>R \<nu> (x r))) (at r within {t0..\<tau>}))"
-    and impls:"\<lceil>P\<rceil> \<le> \<lceil>\<lambda>s. \<theta> s = 0\<rceil>" "\<lceil>\<lambda>s. \<theta> s = 0\<rceil> \<le> \<lceil>Q\<rceil>" "\<lceil>G\<rceil> \<le> \<lceil>\<lambda>s. \<nu> s = 0\<rceil>" and "t0 \<le> t"
+  assumes "I is_ode_invariant_of f {t0..t} S" 
+    and "t0 \<le> t" and "\<lceil>P\<rceil> \<le> \<lceil>I\<rceil>" and "\<lceil>I\<rceil> \<le> \<lceil>Q\<rceil>"
   shows "\<lceil>P\<rceil> \<le> wp ({[x\<acute>=f]{t0..t} S @ t0 & G}) \<lceil>Q\<rceil>"
-  apply(rule_tac C="\<lambda>s. \<theta> s = 0" in dCut_interval, simp add: \<open>t0 \<le> t\<close>)
-   apply(subgoal_tac "\<lceil>\<lambda>s. \<theta> s = 0\<rceil> \<le> wp ({[x\<acute>=f]{t0..t} S @ t0 & G}) \<lceil>\<lambda>s. \<theta> s = 0\<rceil>")
-  using impls apply(subst (asm) wp_nd_fun, subst wp_nd_fun) apply auto[1]
-   apply(rule_tac \<nu>="\<nu>" in invariant_eq_0_interval)
-  using assms(1,4,5) apply(simp, simp, simp)
-  apply(rule dWeakening) using impls by auto
-
-lemma invariant_geq_0:
-  fixes \<theta>::"'a::banach \<Rightarrow> real"
-  assumes nuHyp:"\<forall> x. (x solves_ode f)T S \<longrightarrow> (\<forall> t \<in> T. \<forall> r \<in> {(Inf T)--t}. 
-  ((\<lambda>\<tau>. \<theta> (x \<tau>)) has_derivative (\<lambda>\<tau>. \<tau> *\<^sub>R (\<nu> (x r)))) (at r within {(Inf T)--t}))"
-    and "\<lceil>G\<rceil> \<le> \<lceil>\<lambda>s. (\<nu> s) \<ge> 0\<rceil>" and "bdd_below T"
-  shows "\<lceil>\<lambda>s. \<theta> s \<ge> 0\<rceil> \<le> wp ({[x\<acute>=f]T S @ (Inf T) & G}) \<lceil>\<lambda>s. \<theta> s \<ge> 0\<rceil>"
-  apply(rule dInvariant [of _ "\<lambda> s. \<nu> s \<ge> 0"])
-  using assms apply(simp, simp add: pderivative_def)
-proof(clarify)
-  fix x and t
-  assume x_ivp:"\<theta> (x (Inf T)) \<ge> 0" "(x solves_ode f) T S" 
-    and tHyp:"t \<in> T" and ge0:"\<forall>r\<in>{Inf T--t}. \<nu> (x r) \<ge> 0"
-  hence "(Inf T) \<le> t" by (simp add: \<open>bdd_below T\<close> cInf_lower) 
-  have "\<forall> r \<in> {(Inf T)--t}. ((\<lambda>\<tau>. \<theta> (x \<tau>)) has_derivative (\<lambda>\<tau>. \<tau> *\<^sub>R (\<nu> (x r)))) 
-    (at r within {(Inf T)--t})" using nuHyp x_ivp(2) and tHyp by auto
-  then have "\<exists>r\<in>{(Inf T)--t}. \<theta> (x t)- \<theta> (x (Inf T)) = (\<lambda>\<tau>. \<tau> *\<^sub>R (\<nu> (x r))) (t - (Inf T))" 
-    by(rule_tac closed_segment_mvt, auto simp: \<open>(Inf T) \<le> t\<close>)
-  from this obtain r where 
-    "r \<in> {(Inf T)--t} \<and> \<theta> (x t)= (t - Inf T) *\<^sub>R \<nu> (x r) + \<theta> (x (Inf T)) " by force 
-  thus "0 \<le> \<theta> (x t)" by (simp add: \<open>Inf T \<le> t\<close> ge0 x_ivp(1))
-qed
-
-corollary invariant_geq_0_interval:
-  fixes \<theta>::"'a::banach \<Rightarrow> real"
-  assumes "\<forall> x. (x solves_ode f){t0..t} S \<longrightarrow> (\<forall> \<tau> \<in> {t0..t}. \<forall> r \<in> {t0..\<tau>}. 
-  ((\<lambda>\<tau>. \<theta> (x \<tau>)) has_derivative (\<lambda>\<tau>. \<tau> *\<^sub>R (\<nu> (x r)))) (at r within {t0..\<tau>}))"
-    and "\<lceil>G\<rceil> \<le> \<lceil>\<lambda>s. \<nu> s \<ge> 0\<rceil>" and "t0 \<le> t"
-  shows "\<lceil>\<lambda>s. \<theta> s \<ge> 0\<rceil> \<le> wp ({[x\<acute>=f]{t0..t} S @ t0 & G}) \<lceil>\<lambda>s. \<theta> s \<ge> 0\<rceil>"
-  apply(subgoal_tac "\<lceil>\<lambda>s. \<theta> s \<ge> 0\<rceil> \<le> wp ({[x\<acute>=f]{t0..t} S @ (Inf {t0..t}) & G}) \<lceil>\<lambda>s. \<theta> s \<ge> 0\<rceil>")
-   apply(subgoal_tac "Inf {t0..t} = t0", simp)
-  using \<open>t0 \<le> t\<close> apply(simp add: closed_segment_eq_real_ivl)
-  apply(rule invariant_geq_0[of _ "{t0..t}" _ _ \<nu>])
-  using assms by(auto simp: closed_segment_eq_real_ivl)
-
-theorem dInvariant_geq_0:
-  fixes \<theta>::"'a::banach \<Rightarrow> real" and \<nu>::"'a \<Rightarrow> real"
-  assumes "\<forall>x. (x solves_ode f) {t0..t} S \<longrightarrow> 
-  (\<forall>\<tau>\<in>{t0..t}. \<forall>r\<in>{t0..\<tau>}. ((\<lambda>\<tau>. \<theta> (x \<tau>)) has_derivative (\<lambda>\<tau>. \<tau> *\<^sub>R \<nu> (x r))) (at r within {t0..\<tau>}))"
-    and impls:"\<lceil>P\<rceil> \<le> \<lceil>\<lambda>s. \<theta> s \<ge> 0\<rceil>" "\<lceil>\<lambda>s. \<theta> s \<ge> 0\<rceil> \<le> \<lceil>Q\<rceil>" "\<lceil>G\<rceil> \<le> \<lceil>\<lambda>s. \<nu> s \<ge> 0\<rceil>" and "t0 \<le> t"
-  shows "\<lceil>P\<rceil> \<le> wp ({[x\<acute>=f]{t0..t} S @ t0 & G}) \<lceil>Q\<rceil>"
-  apply(rule_tac C="\<lambda>s. \<theta> s \<ge> 0" in dCut_interval, simp add: \<open>t0 \<le> t\<close>)
-   apply(subgoal_tac "\<lceil>\<lambda>s. \<theta> s \<ge> 0\<rceil> \<le> wp ({[x\<acute>=f]{t0..t} S @ t0 & G}) \<lceil>\<lambda>s. \<theta> s \<ge> 0\<rceil>")
-  using impls apply(subst (asm) wp_nd_fun, subst wp_nd_fun) apply auto[1]
-  apply(rule_tac \<nu>="\<nu>" in invariant_geq_0_interval)
-  using assms(1,4,5) apply(simp, simp, simp)
-  apply(rule dWeakening) using impls by auto
-
-lemma invariant_leq_0:
-  fixes \<theta>::"'a::banach \<Rightarrow> real"
-  assumes nuHyp:"\<forall> x. (x solves_ode f)T S \<longrightarrow> (\<forall> t \<in> T. \<forall> r \<in> {(Inf T)--t}. 
-  ((\<lambda>\<tau>. \<theta> (x \<tau>)) has_derivative (\<lambda>\<tau>. \<tau> *\<^sub>R (\<nu> (x r)))) (at r within {(Inf T)--t}))"
-    and "\<lceil>G\<rceil> \<le> \<lceil>\<lambda>s. (\<nu> s) \<le> 0\<rceil>" and "bdd_below T"
-  shows "\<lceil>\<lambda>s. \<theta> s \<le> 0\<rceil> \<le> wp ({[x\<acute>=f]T S @ (Inf T) & G}) \<lceil>\<lambda>s. \<theta> s \<le> 0\<rceil>"
-  apply(rule dInvariant [of _ "\<lambda> s. \<nu> s \<le> 0"])
-  using assms apply(simp, simp add: pderivative_def)
-proof(clarify)
-  fix x and t
-  assume x_ivp:"\<theta> (x (Inf T)) \<le> 0" "(x solves_ode f) T S" 
-    and tHyp:"t \<in> T" and ge0:"\<forall>r\<in>{Inf T--t}. \<nu> (x r) \<le> 0"
-  hence "(Inf T) \<le> t" by (simp add: \<open>bdd_below T\<close> cInf_lower) 
-  have "\<forall> r \<in> {(Inf T)--t}. ((\<lambda>\<tau>. \<theta> (x \<tau>)) has_derivative (\<lambda>\<tau>. \<tau> *\<^sub>R (\<nu> (x r)))) 
-    (at r within {(Inf T)--t})" using nuHyp x_ivp(2) and tHyp by auto
-  then have "\<exists>r\<in>{(Inf T)--t}. \<theta> (x t)- \<theta> (x (Inf T)) = (\<lambda>\<tau>. \<tau> *\<^sub>R (\<nu> (x r))) (t - (Inf T))" 
-    by(rule_tac closed_segment_mvt, auto simp: \<open>(Inf T) \<le> t\<close>)
-  from this obtain r where 
-    "r \<in> {(Inf T)--t} \<and> \<theta> (x t)= (t - Inf T) *\<^sub>R \<nu> (x r) + \<theta> (x (Inf T))" by force 
-  thus "\<theta> (x t) \<le> 0" using \<open>(Inf T) \<le> t\<close> ge0 x_ivp(1)
-    by (metis add_decreasing2 ge_iff_diff_ge_0 split_scaleR_neg_le)
-qed
-
-corollary invariant_leq_0_interval:
-  fixes \<theta>::"'a::banach \<Rightarrow> real"
-  assumes "\<forall> x. (x solves_ode f){t0..t} S \<longrightarrow> (\<forall> \<tau> \<in> {t0..t}. \<forall> r \<in> {t0..\<tau>}. 
-  ((\<lambda>\<tau>. \<theta> (x \<tau>)) has_derivative (\<lambda>\<tau>. \<tau> *\<^sub>R (\<nu> (x r)))) (at r within {t0..\<tau>}))"
-    and "\<lceil>G\<rceil> \<le> \<lceil>\<lambda>s. \<nu> s \<le> 0\<rceil>" and "t0 \<le> t"
-  shows "\<lceil>\<lambda>s. \<theta> s \<le> 0\<rceil> \<le> wp ({[x\<acute>=f]{t0..t} S @ t0 & G}) \<lceil>\<lambda>s. \<theta> s \<le> 0\<rceil>"
-  apply(subgoal_tac "\<lceil>\<lambda>s. \<theta> s \<le> 0\<rceil> \<le> wp ({[x\<acute>=f]{t0..t} S @ (Inf {t0..t}) & G}) \<lceil>\<lambda>s. \<theta> s \<le> 0\<rceil>")
-   apply(subgoal_tac "Inf {t0..t} = t0", simp)
-  using \<open>t0 \<le> t\<close> apply(simp add: closed_segment_eq_real_ivl)
-  apply(rule invariant_leq_0[of _ "{t0..t}" _ _ \<nu>])
-  using assms by(auto simp: closed_segment_eq_real_ivl)
-
-theorem dInvariant_leq_0:
-  fixes \<theta>::"'a::banach \<Rightarrow> real" and \<nu>::"'a \<Rightarrow> real"
-  assumes "\<forall>x. (x solves_ode f) {t0..t} S \<longrightarrow> 
-  (\<forall>\<tau>\<in>{t0..t}. \<forall>r\<in>{t0..\<tau>}. ((\<lambda>\<tau>. \<theta> (x \<tau>)) has_derivative (\<lambda>\<tau>. \<tau> *\<^sub>R \<nu> (x r))) (at r within {t0..\<tau>}))"
-    and impls:"\<lceil>P\<rceil> \<le> \<lceil>\<lambda>s. \<theta> s \<le> 0\<rceil>" "\<lceil>\<lambda>s. \<theta> s \<le> 0\<rceil> \<le> \<lceil>Q\<rceil>" "\<lceil>G\<rceil> \<le> \<lceil>\<lambda>s. \<nu> s \<le> 0\<rceil>" and "t0 \<le> t"
-  shows "\<lceil>P\<rceil> \<le> wp ({[x\<acute>=f]{t0..t} S @ t0 & G}) \<lceil>Q\<rceil>"
-  apply(rule_tac C="\<lambda>s. \<theta> s \<le> 0" in dCut_interval, simp add: \<open>t0 \<le> t\<close>)
-   apply(subgoal_tac "\<lceil>\<lambda>s. \<theta> s \<le> 0\<rceil> \<le> wp ({[x\<acute>=f]{t0..t} S @ t0 & G}) \<lceil>\<lambda>s. \<theta> s \<le> 0\<rceil>")
-  using impls apply(subst (asm) wp_nd_fun, subst wp_nd_fun) apply auto[1]
-  apply(rule_tac \<nu>="\<nu>" in invariant_leq_0_interval)
-  using assms(1,4,5) apply(simp, simp, simp)
-  apply(rule dWeakening) using impls by auto
-
-lemma invariant_above_0:
-  fixes \<theta>::"'a::banach \<Rightarrow> real"
-  assumes nuHyp:"\<forall> x. (x solves_ode f)T S \<longrightarrow>  (\<forall> t \<in> T. \<forall> r \<in> {(Inf T)--t}. 
-  ((\<lambda>\<tau>. \<theta> (x \<tau>)) has_derivative (\<lambda>\<tau>. \<tau> *\<^sub>R (\<nu> (x r)))) (at r within {(Inf T)--t}))"
-    and "\<lceil>G\<rceil> \<le> \<lceil>\<lambda>s. (\<nu> s) \<ge> 0\<rceil>" and "bdd_below T"
-  shows "\<lceil>\<lambda>s. \<theta> s > 0\<rceil> \<le> wp ({[x\<acute>=f]T S @ (Inf T) & G}) \<lceil>\<lambda>s. \<theta> s > 0\<rceil>"
-  apply(rule dInvariant [of _ "\<lambda> s. \<nu> s \<ge> 0"])
-  using assms apply(simp, simp add: pderivative_def)
-proof(clarify)
-  fix x and t
-  assume x_ivp:"(x solves_ode f) T S" "\<theta> (x (Inf T)) > 0"
-    and tHyp:"t \<in> T" and ge0:"\<forall>r\<in>{Inf T--t}. \<nu> (x r) \<ge> 0"
-  hence "(Inf T) \<le> t" by (simp add: \<open>bdd_below T\<close> cInf_lower) 
-  have "\<forall> r \<in> {(Inf T)--t}. ((\<lambda>\<tau>. \<theta> (x \<tau>)) has_derivative (\<lambda>\<tau>. \<tau> *\<^sub>R (\<nu> (x r)))) 
-    (at r within {(Inf T)--t})" using nuHyp x_ivp(1) and tHyp by auto
-  then have "\<exists>r\<in>{(Inf T)--t}. \<theta> (x t)- \<theta> (x (Inf T)) = (\<lambda>\<tau>. \<tau> *\<^sub>R (\<nu> (x r))) (t - (Inf T))" 
-    by(rule_tac closed_segment_mvt, auto simp: \<open>(Inf T) \<le> t\<close>)
-  from this obtain r where 
-    "r \<in> {(Inf T)--t} \<and> \<theta> (x t)= (t - Inf T) *\<^sub>R \<nu> (x r) + \<theta> (x (Inf T)) " by force 
-  thus "0 < \<theta> (x t)"  
-    by (metis \<open>(Inf T) \<le> t\<close> ge0 x_ivp(2) Groups.add_ac(2) add_mono_thms_linordered_field(3) 
-        ge_iff_diff_ge_0 monoid_add_class.add_0_right scaleR_nonneg_nonneg)
-qed
-
-corollary invariant_above_0_interval:
-  fixes \<theta>::"'a::banach \<Rightarrow> real"
-  assumes "\<forall> x. (x solves_ode f){t0..t} S \<longrightarrow> (\<forall> \<tau> \<in> {t0..t}. \<forall> r \<in> {t0..\<tau>}. 
-  ((\<lambda>\<tau>. \<theta> (x \<tau>)) has_derivative (\<lambda>\<tau>. \<tau> *\<^sub>R (\<nu> (x r)))) (at r within {t0..\<tau>}))"
-    and "\<lceil>G\<rceil> \<le> \<lceil>\<lambda>s. \<nu> s \<ge> 0\<rceil>" and "t0 \<le> t"
-  shows "\<lceil>\<lambda>s. \<theta> s > 0\<rceil> \<le> wp ({[x\<acute>=f]{t0..t} S @ t0 & G}) \<lceil>\<lambda>s. \<theta> s > 0\<rceil>"
-  apply(subgoal_tac "\<lceil>\<lambda>s. \<theta> s > 0\<rceil> \<le> wp ({[x\<acute>=f]{t0..t} S @ (Inf {t0..t}) & G}) \<lceil>\<lambda>s. \<theta> s > 0\<rceil>")
-   apply(subgoal_tac "Inf {t0..t} = t0", simp)
-  using \<open>t0 \<le> t\<close> apply(simp add: closed_segment_eq_real_ivl)
-  apply(rule invariant_above_0[of _ "{t0..t}" _ _ \<nu>])
-  using assms by(auto simp: closed_segment_eq_real_ivl)
-
-theorem dInvariant_above_0:
-  fixes \<theta>::"'a::banach \<Rightarrow> real" and \<nu>::"'a \<Rightarrow> real"
-  assumes "\<forall>x. (x solves_ode f) {t0..t} S \<longrightarrow> 
-  (\<forall>\<tau>\<in>{t0..t}. \<forall>r\<in>{t0..\<tau>}. ((\<lambda>\<tau>. \<theta> (x \<tau>)) has_derivative (\<lambda>\<tau>. \<tau> *\<^sub>R \<nu> (x r))) (at r within {t0..\<tau>}))"
-    and impls:"\<lceil>P\<rceil> \<le> \<lceil>\<lambda>s. \<theta> s > 0\<rceil>" "\<lceil>\<lambda>s. \<theta> s > 0\<rceil> \<le> \<lceil>Q\<rceil>" "\<lceil>G\<rceil> \<le> \<lceil>\<lambda>s. \<nu> s \<ge> 0\<rceil>" and "t0 \<le> t"
-  shows "\<lceil>P\<rceil> \<le> wp ({[x\<acute>=f]{t0..t} S @ t0 & G}) \<lceil>Q\<rceil>"
-  apply(rule_tac C="\<lambda>s. \<theta> s > 0" in dCut_interval, simp add: \<open>t0 \<le> t\<close>)
-   apply(subgoal_tac "\<lceil>\<lambda>s. \<theta> s > 0\<rceil> \<le> wp ({[x\<acute>=f]{t0..t} S @ t0 & G}) \<lceil>\<lambda>s. \<theta> s > 0\<rceil>")
-  using impls apply(subst (asm) wp_nd_fun, subst wp_nd_fun) apply auto[1]
-  apply(rule_tac \<nu>="\<nu>" in invariant_above_0_interval)
-  using assms(1,4,5) apply(simp, simp, simp)
-  apply(rule dWeakening) using impls  by auto
-
-lemma invariant_below_0:
-  fixes \<theta>::"'a::banach \<Rightarrow> real"
-  assumes nuHyp:"\<forall> x. (x solves_ode f)T S \<longrightarrow>  (\<forall> t \<in> T. \<forall> r \<in> {(Inf T)--t}. 
-  ((\<lambda>\<tau>. \<theta> (x \<tau>)) has_derivative (\<lambda>\<tau>. \<tau> *\<^sub>R (\<nu> (x r)))) (at r within {(Inf T)--t}))"
-    and "\<lceil>G\<rceil> \<le> \<lceil>\<lambda>s. (\<nu> s) \<le> 0\<rceil>" and "bdd_below T"
-  shows "\<lceil>\<lambda>s. \<theta> s < 0\<rceil> \<le> wp ({[x\<acute>=f]T S @ (Inf T) & G}) \<lceil>\<lambda>s. \<theta> s < 0\<rceil>"
-  apply(rule dInvariant [of _ "\<lambda> s. \<nu> s \<le> 0"])
-  using assms apply(simp, simp add: pderivative_def)
-proof(clarify)
-  fix x and t
-  assume x_ivp:"(x solves_ode f) T S" "\<theta> (x (Inf T)) < 0"
-    and tHyp:"t \<in> T" and ge0:"\<forall>r\<in>{Inf T--t}. \<nu> (x r) \<le> 0"
-  hence "(Inf T) \<le> t" by (simp add: \<open>bdd_below T\<close> cInf_lower) 
-  have "\<forall> r \<in> {(Inf T)--t}. ((\<lambda>\<tau>. \<theta> (x \<tau>)) has_derivative (\<lambda>\<tau>. \<tau> *\<^sub>R (\<nu> (x r)))) 
-    (at r within {(Inf T)--t})" using nuHyp x_ivp(1) and tHyp by auto
-  then have "\<exists>r\<in>{(Inf T)--t}. \<theta> (x t)- \<theta> (x (Inf T)) = (\<lambda>\<tau>. \<tau> *\<^sub>R (\<nu> (x r))) (t - (Inf T))" 
-    by(rule_tac closed_segment_mvt, auto simp: \<open>(Inf T) \<le> t\<close>)
-  thus "\<theta> (x t) < 0"  using \<open>(Inf T) \<le> t\<close> ge0 x_ivp(2)
-    by (metis add_mono_thms_linordered_field(3) diff_gt_0_iff_gt ge_iff_diff_ge_0 linorder_not_le 
-        monoid_add_class.add_0_left monoid_add_class.add_0_right split_scaleR_neg_le) 
-qed
-
-corollary invariant_below_0_interval:
-  fixes \<theta>::"'a::banach \<Rightarrow> real"
-  assumes "\<forall> x. (x solves_ode f){t0..t} S \<longrightarrow> (\<forall> \<tau> \<in> {t0..t}. \<forall> r \<in> {t0..\<tau>}. 
-  ((\<lambda>\<tau>. \<theta> (x \<tau>)) has_derivative (\<lambda>\<tau>. \<tau> *\<^sub>R (\<nu> (x r)))) (at r within {t0..\<tau>}))"
-    and "\<lceil>G\<rceil> \<le> \<lceil>\<lambda>s. \<nu> s \<le> 0\<rceil>" and "t0 \<le> t"
-  shows "\<lceil>\<lambda>s. \<theta> s < 0\<rceil> \<le> wp ({[x\<acute>=f]{t0..t} S @ t0 & G}) \<lceil>\<lambda>s. \<theta> s < 0\<rceil>"
-  apply(subgoal_tac "\<lceil>\<lambda>s. \<theta> s < 0\<rceil> \<le> wp ({[x\<acute>=f]{t0..t} S @ (Inf {t0..t}) & G}) \<lceil>\<lambda>s. \<theta> s < 0\<rceil>")
-   apply(subgoal_tac "Inf {t0..t} = t0", simp)
-  using \<open>t0 \<le> t\<close> apply(simp add: closed_segment_eq_real_ivl)
-  apply(rule invariant_below_0[of _ "{t0..t}" _ _ \<nu>])
-  using assms by(auto simp: closed_segment_eq_real_ivl)
-
-theorem dInvariant_below_0:
-  fixes \<theta>::"'a::banach \<Rightarrow> real"
-  assumes "\<forall>x. (x solves_ode f) {t0..t} S \<longrightarrow> 
-  (\<forall>\<tau>\<in>{t0..t}. \<forall>r\<in>{t0..\<tau>}. ((\<lambda>\<tau>. \<theta> (x \<tau>)) has_derivative (\<lambda>\<tau>. \<tau> *\<^sub>R \<nu> (x r))) (at r within {t0..\<tau>}))"
-    and impls:"\<lceil>P\<rceil> \<le> \<lceil>\<lambda>s. \<theta> s < 0\<rceil>" "\<lceil>\<lambda>s. \<theta> s < 0\<rceil> \<le> \<lceil>Q\<rceil>" "\<lceil>G\<rceil> \<le> \<lceil>\<lambda>s. \<nu> s \<le> 0\<rceil>" and "t0 \<le> t"
-  shows "\<lceil>P\<rceil> \<le> wp ({[x\<acute>=f]{t0..t} S @ t0 & G}) \<lceil>Q\<rceil>"
-  using \<open>t0 \<le> t\<close> apply(rule_tac C="\<lambda>s. \<theta> s < 0" in dCut_interval, simp add: \<open>t0 \<le> t\<close>)
-   apply(subgoal_tac "\<lceil>\<lambda>s. \<theta> s < 0\<rceil> \<le> wp ({[x\<acute>=f]{t0..t} S @ t0 & G}) \<lceil>\<lambda>s. \<theta> s < 0\<rceil>")
-  using impls apply(subst (asm) wp_nd_fun, subst wp_nd_fun) apply auto[1]
-  apply(rule_tac \<nu>="\<nu>" in invariant_below_0_interval)
-  using assms(1,4,5) apply(simp, simp, simp)
-  apply(rule dWeakening) using impls by auto
-
-lemma invariant_meet:
-  assumes "\<lceil>I1\<rceil> \<le> wp ({[x\<acute>=f]T S @ t0 & G}) \<lceil>I1\<rceil>"
-    and "\<lceil>I2\<rceil> \<le> wp ({[x\<acute>=f]T S @ t0 & G}) \<lceil>I2\<rceil>"
-  shows "\<lceil>\<lambda>s. I1 s \<and> I2 s\<rceil> \<le> wp ({[x\<acute>=f]T S @ t0 & G}) \<lceil>\<lambda>s. I1 s \<and> I2 s\<rceil>"
-  using assms by(subst (asm) wp_nd_fun, subst (asm) wp_nd_fun, subst wp_nd_fun, simp, blast)
-
-theorem dInvariant_meet:
-  assumes "\<lceil>I1\<rceil> \<le> wp ({[x\<acute>=f]{t0..t} S @ t0 & G}) \<lceil>I1\<rceil>" and "\<lceil>I2\<rceil> \<le> wp ({[x\<acute>=f]{t0..t} S @ t0 & G}) \<lceil>I2\<rceil>"
-    and impls:"\<lceil>P\<rceil> \<le> \<lceil>\<lambda>s. I1 s \<and> I2 s\<rceil>" "\<lceil>\<lambda>s. I1 s \<and> I2 s\<rceil> \<le> \<lceil>Q\<rceil>" and "t0 \<le> t"
-  shows "\<lceil>P\<rceil> \<le> wp ({[x\<acute>=f]{t0..t} S @ t0 & G}) \<lceil>Q\<rceil>"
-  apply(rule_tac C="\<lambda>s. I1 s \<and> I2 s" in dCut_interval, simp add: \<open>t0 \<le> t\<close>)
-   apply(subgoal_tac "\<lceil>\<lambda>s. I1 s \<and> I2 s\<rceil> \<le> wp ({[x\<acute>=f]{t0..t} S @ t0 & G}) \<lceil>\<lambda>s. I1 s \<and> I2 s\<rceil>")
-  using impls apply(transfer, simp add: le_fun_def) apply auto[1]
-    apply(rule invariant_meet)
-  using assms(1,2,5) apply(simp, simp)
+  using assms(1) apply(rule_tac C="I" in dCut)
+    apply(simp add: \<open>t0 \<le> t\<close>)
+   apply(drule_tac G="G" in dInvariant)
+  using assms(3,4) dual_order.trans apply blast 
   apply(rule dWeakening)
-  using impls by simp
+  using assms by auto
 
-lemma invariant_join:
-  assumes "\<lceil>I1\<rceil> \<le> wp ({[x\<acute>=f]T S @ t0 & G}) \<lceil>I1\<rceil>"
-    and "\<lceil>I2\<rceil> \<le> wp ({[x\<acute>=f]T S @ t0 & G}) \<lceil>I2\<rceil>"
-  shows "\<lceil>\<lambda>s. I1 s \<or> I2 s\<rceil> \<le> wp ({[x\<acute>=f]T S @ t0 & G}) \<lceil>\<lambda>s. I1 s \<or> I2 s\<rceil>"
-  using assms by(subst (asm) wp_nd_fun, subst (asm) wp_nd_fun, subst wp_nd_fun, simp)
+text{* Finally, we obtain some conditions to prove specific instances of differential invariants. *}
 
-theorem dInvariant_join:
-  assumes "\<lceil>I1\<rceil> \<le> wp ({[x\<acute>=f]{t0..t} S @ t0 & G}) \<lceil>I1\<rceil>" and "\<lceil>I2\<rceil> \<le> wp ({[x\<acute>=f]{t0..t} S @ t0 & G}) \<lceil>I2\<rceil>"
-    and impls:"\<lceil>P\<rceil> \<le> \<lceil>\<lambda>s. I1 s \<or> I2 s\<rceil>" "\<lceil>\<lambda>s. I1 s \<or> I2 s\<rceil> \<le> \<lceil>Q\<rceil>" and "t0 \<le> t"
-  shows "\<lceil>P\<rceil> \<le> wp ({[x\<acute>=f]{t0..t} S @ t0 & G}) \<lceil>Q\<rceil>"
-  apply(rule_tac C="\<lambda>s. I1 s \<or> I2 s" in dCut_interval, simp add: \<open>t0 \<le> t\<close>)
-   apply(subgoal_tac "\<lceil>\<lambda>s. I1 s \<or> I2 s\<rceil> \<le> wp ({[x\<acute>=f]{t0..t} S @ t0 & G}) \<lceil>\<lambda>s. I1 s \<or> I2 s\<rceil>")
-  using impls apply(transfer, simp add: le_fun_def) apply auto[1]
-    apply(rule invariant_join)
-  using assms(1,2,5) apply(simp, simp)
-  apply(rule dWeakening)
-  using impls by auto
+named_theorems ode_invariant_rules "compilation of rules for differential invariants."
+
+lemma [ode_invariant_rules]:
+fixes \<theta>::"'a::banach \<Rightarrow> real"
+assumes "\<forall> x. (x solves_ode f){t0..t} S \<longrightarrow> (\<forall> \<tau> \<in> {t0..t}. \<forall> r \<in> {t0--\<tau>}. 
+  ((\<lambda>\<tau>. \<theta> (x \<tau>) - \<nu> (x \<tau>) ) has_derivative (\<lambda>\<tau>.  \<tau> *\<^sub>R 0)) (at r within {t0--\<tau>}))"
+shows "(\<lambda>s. \<theta> s = \<nu> s) is_ode_invariant_of f {t0..t} S"
+proof(simp add: ode_invariant_def, clarsimp)
+fix x \<tau> assume x_ivp:"(x solves_ode f){t0..t} S" "\<theta> (x t0) = \<nu> (x t0)" and tHyp:"t0 \<le> \<tau>" "\<tau> \<le> t"
+  from this and assms have "\<forall> r \<in> {t0--\<tau>}. ((\<lambda>\<tau>. \<theta> (x \<tau>) - \<nu> (x \<tau>) ) has_derivative 
+  (\<lambda>\<tau>.  \<tau> *\<^sub>R 0)) (at r within {t0--\<tau>})" by auto
+  then have "\<exists>r\<in>{t0--\<tau>}. (\<theta> (x \<tau>) - \<nu> (x \<tau>)) - (\<theta> (x t0) - \<nu> (x t0)) = 
+  (\<lambda>\<tau>. \<tau> *\<^sub>R 0) (\<tau> - t0)" by(rule_tac closed_segment_mvt, auto simp: tHyp) 
+  thus "\<theta> (x \<tau>) = \<nu> (x \<tau>)" by (simp add: x_ivp(2))
+qed
+
+lemma [ode_invariant_rules]:
+fixes \<theta>::"'a::banach \<Rightarrow> real"
+assumes "\<forall> x. (x solves_ode f){t0..t} S \<longrightarrow> (\<forall> \<tau> \<in> {t0..t}. \<forall> r \<in> {t0--\<tau>}. \<theta>' (x r) \<ge> \<nu>' (x r)
+\<and> ((\<lambda>\<tau>. \<theta> (x \<tau>) - \<nu> (x \<tau>)) has_derivative (\<lambda>\<tau>. \<tau> *\<^sub>R  (\<theta>' (x r) -  \<nu>' (x r)))) (at r within {t0--\<tau>}))"
+shows "(\<lambda>s. \<nu> s \<le> \<theta> s) is_ode_invariant_of f {t0..t} S"
+proof(simp add: ode_invariant_def, clarsimp)
+fix x \<tau> assume x_ivp:"(x solves_ode f){t0..t} S" "\<nu> (x t0) \<le> \<theta> (x t0)" and tHyp:"t0 \<le> \<tau>" "\<tau> \<le> t"
+  from this and assms have primed:"\<forall> r \<in> {t0--\<tau>}. ((\<lambda>\<tau>. \<theta> (x \<tau>) - \<nu> (x \<tau>)) has_derivative 
+(\<lambda>\<tau>. \<tau> *\<^sub>R  (\<theta>' (x r) -  \<nu>' (x r)))) (at r within {t0--\<tau>}) \<and> \<theta>' (x r) \<ge> \<nu>' (x r)" by auto
+  then have "\<exists>r\<in>{t0--\<tau>}. (\<theta> (x \<tau>) - \<nu> (x \<tau>)) - (\<theta> (x t0) - \<nu> (x t0)) = 
+  (\<lambda>\<tau>. \<tau> *\<^sub>R (\<theta>' (x r) -  \<nu>' (x r))) (\<tau> - t0)" by(rule_tac closed_segment_mvt, auto simp: \<open>t0 \<le> \<tau>\<close>)
+  from this obtain r where "r \<in> {t0--\<tau>}" and 
+    "\<theta> (x \<tau>) - \<nu> (x \<tau>) = (\<tau> - t0) *\<^sub>R (\<theta>' (x r) -  \<nu>' (x r)) + (\<theta> (x t0) - \<nu> (x t0))" by force 
+  also have "... \<ge> 0" using tHyp(1) x_ivp(2) primed by (simp add: calculation(1))  
+  ultimately show "\<nu> (x \<tau>) \<le> \<theta> (x \<tau>)" by simp
+qed
+
+lemma [ode_invariant_rules]:
+fixes \<theta>::"'a::banach \<Rightarrow> real"
+assumes "\<forall> x. (x solves_ode f){t0..t} S \<longrightarrow> (\<forall> \<tau> \<in> {t0..t}. \<forall> r \<in> {t0--\<tau>}. \<theta>' (x r) \<ge> \<nu>' (x r)
+\<and> ((\<lambda>\<tau>. \<theta> (x \<tau>) - \<nu> (x \<tau>)) has_derivative (\<lambda>\<tau>. \<tau> *\<^sub>R  (\<theta>' (x r) -  \<nu>' (x r)))) (at r within {t0--\<tau>}))"
+shows "(\<lambda>s. \<nu> s < \<theta> s) is_ode_invariant_of f {t0..t} S"
+proof(simp add: ode_invariant_def, clarsimp)
+fix x \<tau> assume x_ivp:"(x solves_ode f){t0..t} S" "\<nu> (x t0) < \<theta> (x t0)" and tHyp:"t0 \<le> \<tau>" "\<tau> \<le> t"
+  from this and assms have primed:"\<forall> r \<in> {t0--\<tau>}. ((\<lambda>\<tau>. \<theta> (x \<tau>) - \<nu> (x \<tau>)) has_derivative 
+(\<lambda>\<tau>. \<tau> *\<^sub>R  (\<theta>' (x r) -  \<nu>' (x r)))) (at r within {t0--\<tau>}) \<and> \<theta>' (x r) \<ge> \<nu>' (x r)" by auto
+  then have "\<exists>r\<in>{t0--\<tau>}. (\<theta> (x \<tau>) - \<nu> (x \<tau>)) - (\<theta> (x t0) - \<nu> (x t0)) = 
+  (\<lambda>\<tau>. \<tau> *\<^sub>R (\<theta>' (x r) -  \<nu>' (x r))) (\<tau> - t0)" by(rule_tac closed_segment_mvt, auto simp: \<open>t0 \<le> \<tau>\<close>)
+  from this obtain r where "r \<in> {t0--\<tau>}" and 
+    "\<theta> (x \<tau>) - \<nu> (x \<tau>) = (\<tau> - t0) *\<^sub>R (\<theta>' (x r) -  \<nu>' (x r)) + (\<theta> (x t0) - \<nu> (x t0))" by force 
+  also have "... > 0" 
+    using tHyp(1) x_ivp(2) primed by (metis (no_types,hide_lams) Groups.add_ac(2) add_sign_intros(1) 
+        calculation(1) diff_gt_0_iff_gt ge_iff_diff_ge_0 less_eq_real_def zero_le_scaleR_iff) 
+  ultimately show "\<nu> (x \<tau>) < \<theta> (x \<tau>)" by simp
+qed
+
+lemma [ode_invariant_rules]:
+fixes \<theta>::"'a::banach \<Rightarrow> real"
+assumes "I1 is_ode_invariant_of f {t0..t} S" and "I2 is_ode_invariant_of f {t0..t} S"
+shows "(\<lambda>s. I1 s \<and> I2 s) is_ode_invariant_of f {t0..t} S"
+  using assms unfolding ode_invariant_def by auto
+
+lemma [ode_invariant_rules]:
+fixes \<theta>::"'a::banach \<Rightarrow> real"
+assumes "I1 is_ode_invariant_of f {t0..t} S" and "I2 is_ode_invariant_of f {t0..t} S"
+shows "(\<lambda>s. I1 s \<or> I2 s) is_ode_invariant_of f {t0..t} S"
+  using assms unfolding ode_invariant_def by auto
 
 end
