HybridVerifVecs/rels/cat2rel_examples.thy
@@ -209,6 +209,108 @@ lemma single_evolution_ball_K:
   apply(subst flow_for_K_DS)
   using assms by(simp_all add: mult_nonneg_nonpos2)
 
+subsubsection{* Circular motion with invariants *}
+
+lemma two_eq_zero: "(2::2) = 0" by simp
+
+lemma [simp]:"i \<noteq> (0::2) \<Longrightarrow> i = 1" using exhaust_2 by fastforce
+
+lemma UNIV_2:"(UNIV::2 set) = {0, 1}"
+  apply safe using exhaust_2 two_eq_zero by auto
+
+lemma sum_axis_UNIV_2[simp]:"(\<Sum>j\<in>(UNIV::2 set). axis i r $ j \<cdot> f j) = r \<cdot> (f::2 \<Rightarrow> real) i"
+  unfolding axis_def UNIV_2 by simp
+
+abbreviation "Circ \<equiv> (\<chi> i. if i= (0::2) then axis (1::2) (- 1::real) else axis 0 1)"
+
+abbreviation "flow_for_Circ t s \<equiv> (\<chi> i. if i= (0::2) then 
+s$0 \<cdot> cos t - s$1 \<cdot> sin t else s$0 \<cdot> sin t + s$1 \<cdot> cos t)"
+
+lemma entries_Circ:"entries Circ = {0, - 1, 1}"
+  apply (simp_all add: axis_def, safe)
+  subgoal by(rule_tac x="0" in exI, simp)+
+  subgoal by(rule_tac x="0" in exI, simp)+
+  by(rule_tac x="1" in exI, simp)+
+
+lemma Circ_is_picard_ivp:"0 \<le> t \<Longrightarrow> t < 1/4 \<Longrightarrow> 
+picard_ivp (\<lambda> t s. Circ *v s) {0..t} UNIV ((real CARD(2))\<^sup>2 \<cdot> maxAbs Circ) 0"
+  apply(rule picard_ivp_linear_system)
+  unfolding entries_Circ by auto
+
+lemma flow_for_Circ_solves_Circ: "((\<lambda> \<tau>. flow_for_Circ \<tau> s) solves_ode (\<lambda>t s.  Circ *v s)) {0..t} UNIV"
+  apply (rule solves_vec_lambda, clarsimp)
+  subgoal for i apply(cases "i=0")
+     apply(simp_all add: matrix_vector_mult_def)
+    unfolding solves_ode_def has_vderiv_on_def has_vector_derivative_def apply auto
+    subgoal for x
+      apply(rule_tac f'1="\<lambda>t. - s$0 \<cdot> (t \<cdot> sin x)" and g'1="\<lambda>t. s$1 \<cdot> (t \<cdot> cos x)"in derivative_eq_intros(11))
+      apply(rule derivative_eq_intros(6)[of cos "(\<lambda>xa. - (xa \<cdot> sin x))"])
+       apply(rule_tac Db1="1" in derivative_eq_intros(58))
+          apply(rule ssubst[of "(\<cdot>) 1" id], force, simp, force, force)
+       apply(rule derivative_eq_intros(6)[of sin "(\<lambda>xa. (xa \<cdot> cos x))"])
+        apply(rule_tac Db1="1" in derivative_eq_intros(55))
+         apply(rule ssubst[of "(\<cdot>) 1" id], force, simp, force, force)
+      by (simp add: Groups.mult_ac(3) Rings.ring_distribs(4))
+    subgoal for x
+      apply(rule_tac f'1="\<lambda>t. s$0 \<cdot> (t \<cdot> cos x)" and g'1="\<lambda>t. - s$1 \<cdot> (t \<cdot> sin x)"in derivative_eq_intros(8))
+      apply(rule derivative_eq_intros(6)[of sin "(\<lambda>xa. xa \<cdot> cos x)"])
+       apply(rule_tac Db1="1" in derivative_eq_intros(55))
+          apply(rule ssubst[of "(\<cdot>) 1" id], force, simp, force, force)
+       apply(rule derivative_eq_intros(6)[of cos "(\<lambda>xa. - (xa \<cdot> sin x))"])
+        apply(rule_tac Db1="1" in derivative_eq_intros(58))
+         apply(rule ssubst[of "(\<cdot>) 1" id], force, simp, force, force)
+      by (simp add: Groups.mult_ac(3) Rings.ring_distribs(4))
+    done
+  done
+
+corollary flow_for_Circ_DS:
+  assumes "0 \<le> t" and "t < 1/4"
+  shows " wp {[x\<acute>=\<lambda> t s. Circ *v s]{0..t} UNIV @ 0 & G} \<lceil>Q\<rceil> = 
+    \<lceil>\<lambda> x. \<forall> \<tau> \<in> {0..t}. (\<forall>r\<in>{0--\<tau>}. G (flow_for_Circ r x)) \<longrightarrow> Q (flow_for_Circ \<tau> x)\<rceil>"
+  apply(subst picard_ivp.wp_g_orbit[of "\<lambda>t s. Circ *v s" _ _ "((real CARD(2))\<^sup>2 \<cdot> maxAbs Circ)" _ 
+"(\<lambda> t x. flow_for_Circ t x)"])
+  using Circ_is_picard_ivp and assms apply blast apply(clarify, rule conjI)
+  using flow_for_Circ_solves_Circ apply blast
+   apply(simp add: vec_eq_iff) using exhaust_2 two_eq_zero apply force 
+  by simp
+
+lemma circular_motion:
+  assumes "0 \<le> t" and "t < 1/4" and "(R::real) > 0"
+  shows"\<lceil>\<lambda>s. R\<^sup>2 = (s $ (0::2))\<^sup>2 + (s $ 1)\<^sup>2\<rceil> \<subseteq> wp 
+  {[x\<acute>=\<lambda>t s. Circ *v s]{0..t} UNIV @ 0 & (\<lambda> s. True)}
+  \<lceil>\<lambda>s. R\<^sup>2 = (s $ (0::2))\<^sup>2 + (s $ 1)\<^sup>2\<rceil>"
+  apply(subst flow_for_Circ_DS)
+  using assms by simp_all
+
+lemma circle_invariant:
+  assumes "0 \<le> t" and "0 < R"
+  shows "(\<lambda>s. R\<^sup>2 = (s $ 0)\<^sup>2 + (s $ 1)\<^sup>2) is_ode_invariant_of (\<lambda>a. ( *v) Circ) {0..t} UNIV"
+  apply(rule_tac ode_invariant_rules, clarsimp)
+  apply(frule_tac i="0" in solves_vec_nth, drule_tac i="1" in solves_vec_nth)
+  apply(unfold solves_ode_def has_vderiv_on_def has_vector_derivative_def, clarsimp)
+  apply(erule_tac x="r" in ballE)+
+    apply(simp add: matrix_vector_mult_def)
+  subgoal for x \<tau> r apply(rule_tac f'1="\<lambda>t. 0" and g'1="\<lambda>t. 0" in derivative_eq_intros(11), simp_all)
+     apply(rule_tac f'1="\<lambda>t. - 2 \<cdot> (x r $ 0) \<cdot> (t \<cdot> x r $ 1)" 
+        and g'1="\<lambda>t. 2 \<cdot> (x r $ 1) \<cdot> t \<cdot> x r $ 0" in derivative_eq_intros(8), simp_all)
+       apply(rule_tac f'1="\<lambda>t. - (t \<cdot> x r $ 1)" in derivative_eq_intros(15))
+        apply(rule_tac t="{0--\<tau>}" and s="{0..t}" in has_derivative_within_subset)
+         apply(simp, simp add: closed_segment_eq_real_ivl, force)
+       apply(rule_tac f'1="\<lambda>t. (t \<cdot> x r $ 0)" in derivative_eq_intros(15))
+        apply(rule_tac t="{0--\<tau>}" and s="{0..t}" in has_derivative_within_subset)
+    by(simp, simp add: closed_segment_eq_real_ivl, force)
+  by(auto simp: closed_segment_eq_real_ivl)
+
+lemma circular_motion_invariants:
+  assumes "0 \<le> t" and "t < 1/4" and "(R::real) > 0"
+  shows"\<lceil>\<lambda>s. R\<^sup>2 = (s $ (0::2))\<^sup>2 + (s $ 1)\<^sup>2\<rceil> \<le> wp 
+  {[x\<acute>=\<lambda>t s. Circ *v s]{0..t} UNIV @ 0 & (\<lambda> s. s $ 0 \<ge> 0)}
+  \<lceil>\<lambda>s. R\<^sup>2 = (s $ (0::2))\<^sup>2 + (s $ 1)\<^sup>2\<rceil>"
+  using assms(1) apply(rule_tac C="\<lambda>s. R\<^sup>2 = (s $ (0::2))\<^sup>2 + (s $ 1)\<^sup>2" in dCut, simp)
+     apply(rule_tac I="\<lambda>s. R\<^sup>2 = (s $ (0::2))\<^sup>2 + (s $ 1)\<^sup>2" in dInvariant')
+  using circle_invariant \<open>R > 0\<close> apply(blast, blast, force, force)
+  by(rule dWeakening, auto)
+
 subsubsection{* Bouncing Ball with solution *}
 text{* Armed now with two vector fields for free-fall kinematics and their respective flows, proving
 the safety of a ``bouncing ball'' is merely an exercise of real arithmetic: *}
@@ -284,16 +386,17 @@ lemma bouncing_ball:
 
 subsubsection{* Bouncing Ball with invariants *}
 
-lemma gravity_is_invariant:"(x solves_ode (\<lambda>t. ( *v) K)) {0..t} UNIV \<Longrightarrow> \<tau> \<in> {0..t} \<Longrightarrow> r \<in> {0..\<tau>} \<Longrightarrow> 
-((\<lambda>\<tau>. x \<tau> $ 2) has_derivative (\<lambda>\<tau>. \<tau> *\<^sub>R 0)) (at r within {0..\<tau>})"
+lemma gravity_is_invariant:"(x solves_ode (\<lambda>t. ( *v) K)) {0..t} UNIV \<Longrightarrow> \<tau> \<in> {0..t} \<Longrightarrow> r \<in> {0--\<tau>} \<Longrightarrow> 
+((\<lambda>\<tau>. - x \<tau> $ 2) has_derivative (\<lambda>\<tau>. \<tau> *\<^sub>R 0)) (at r within {0--\<tau>})"
   apply(drule_tac i="2" in solves_vec_nth)
   apply(unfold solves_ode_def has_vderiv_on_def has_vector_derivative_def, clarify)
   apply(erule_tac x="r" in ballE, simp add: matrix_vector_mult_def)
-  by (simp_all add: has_derivative_within_subset)
+   apply(rule_tac f'1="\<lambda>s. 0" in derivative_eq_intros(10))
+  by(auto simp: closed_segment_eq_real_ivl has_derivative_within_subset)
 
 lemma bouncing_ball_invariant:"(x solves_ode (\<lambda>t. ( *v) K)) {0..t} UNIV \<Longrightarrow> \<tau> \<in> {0..t} \<Longrightarrow> 
-r \<in> {0..\<tau>} \<Longrightarrow> ((\<lambda>\<tau>. 2 \<cdot> x \<tau> $ 2 \<cdot> x \<tau> $ 0 - 2 \<cdot> x \<tau> $ 2 \<cdot> H - x \<tau> $ 1 \<cdot> x \<tau> $ 1) has_derivative 
-(\<lambda>\<tau>. \<tau> *\<^sub>R 0)) (at r within {0..\<tau>})"
+r \<in> {0--\<tau>} \<Longrightarrow> ((\<lambda>\<tau>. 2 \<cdot> x \<tau> $ 2 \<cdot> x \<tau> $ 0 - 2 \<cdot> x \<tau> $ 2 \<cdot> H - x \<tau> $ 1 \<cdot> x \<tau> $ 1) has_derivative 
+(\<lambda>\<tau>. \<tau> *\<^sub>R 0)) (at r within {0--\<tau>})"
   apply(frule_tac i="2" in solves_vec_nth,frule_tac i="1" in solves_vec_nth,drule_tac i="0" in solves_vec_nth)
   apply(unfold solves_ode_def has_vderiv_on_def has_vector_derivative_def, clarify)
   apply(erule_tac x="r" in ballE, simp_all add: matrix_vector_mult_def)+
@@ -301,7 +404,8 @@ r \<in> {0..\<tau>} \<Longrightarrow> ((\<lambda>\<tau>. 2 \<cdot> x \<tau> $ 2 
       and g'1="\<lambda>t. 2 \<cdot> (t \<cdot> (x r $ 1 \<cdot> x r $ 2))" in derivative_eq_intros(11))
     apply(rule_tac f'1="\<lambda>t. 2 \<cdot> x r $ 2 \<cdot> (t \<cdot> x r $ 1)" and g'1="\<lambda>t. 0" in derivative_eq_intros(11))
       apply(rule_tac f'1="\<lambda>t. 0" and g'1="(\<lambda>xa. xa \<cdot> x r $ 1)" in derivative_eq_intros(12))
-        apply(rule_tac g'1="\<lambda>t. 0" in derivative_eq_intros(6), simp_all add: has_derivative_within_subset)
+           apply(rule_tac g'1="\<lambda>t. 0" in derivative_eq_intros(6))
+            apply(simp_all add: has_derivative_within_subset closed_segment_eq_real_ivl)
   apply(rule_tac g'1="\<lambda>t. 0" in derivative_eq_intros(7))
     apply(rule_tac g'1="\<lambda>t. 0" in derivative_eq_intros(6), simp_all add: has_derivative_within_subset)
   by(rule_tac f'1="(\<lambda>xa. xa \<cdot> x r $ 2)" and g'1="(\<lambda>xa. xa \<cdot> x r $ 2)" in derivative_eq_intros(12), 
@@ -316,112 +420,17 @@ lemma bouncing_ball_invariants:
   apply(rule_tac I="\<lceil>\<lambda>s. 0 \<le> s$0 \<and> 0 > s$2 \<and> 2 \<cdot> s$2 \<cdot> s$0 = 2 \<cdot> s$2 \<cdot> H + (s$1 \<cdot> s$1)\<rceil>" in rel_ad_mka_starI)
     apply(simp, simp only: rel_antidomain_kleene_algebra.fbox_seq)
    apply(subst p2r_r2p_wp_sym[of "(IF (\<lambda>s. s $ 0 = 0) THEN ([1 ::== (\<lambda>s. - s $ 1)]) ELSE Id FI)"])
-  using assms(1) apply(rule dCut_interval[of _ _ _ _ _ _ "\<lambda> s. s $ 2 < 0"])
-   apply(rule_tac \<theta>="\<lambda>s. s $ 2" and \<nu>="\<lambda>s. 0" in dInvariant_below_0)
-  using gravity_is_invariant apply force
-       apply(simp, simp, simp, simp add: \<open>0 \<le> t\<close>)
-   apply(rule_tac C="\<lambda> s. 2 \<cdot> s$2 \<cdot> s$0 - 2 \<cdot> s$2 \<cdot> H - s$1 \<cdot> s$1 = 0" in dCut_interval, simp add: \<open>0 \<le> t\<close>)
-   apply(rule_tac \<theta>="\<lambda>s. 2 \<cdot> s$2 \<cdot> s$0 - 2 \<cdot> s$2 \<cdot> H - s$1 \<cdot> s$1" and \<nu>="\<lambda> s. 0" in dInvariant_eq_0)
-  using bouncing_ball_invariant apply force
-  apply(simp, simp, simp, simp add: \<open>0 \<le> t\<close>)
+ using assms(1) apply(rule dCut[of _ _ _ _ _ _ "\<lambda> s. s $ 2 < 0"])
+    apply(rule_tac I="\<lambda> s. s $ 2 < 0" in dInvariant')
+       apply(rule_tac \<theta>'="\<lambda>s. 0" and \<nu>'="\<lambda>s. 0" in ode_invariant_rules(3))
+  using gravity_is_invariant apply(force, simp add: \<open>0 \<le> t\<close>, simp, simp)
+   apply(rule_tac C="\<lambda> s. 2 \<cdot> s$2 \<cdot> s$0 - 2 \<cdot> s$2 \<cdot> H - s$1 \<cdot> s$1 = 0" in dCut, simp add: \<open>0 \<le> t\<close>)
+    apply(rule_tac I="\<lambda> s. 2 \<cdot> s$2 \<cdot> s$0 - 2 \<cdot> s$2 \<cdot> H - s$1 \<cdot> s$1 = 0" in dInvariant')
+  apply(rule ode_invariant_rules)
+  using bouncing_ball_invariant apply(force, simp add: \<open>0 \<le> t\<close>, simp, simp)
    apply(rule dWeakening, subst p2r_r2p_wp)
-  unfolding rel_antidomain_kleene_algebra.cond_def rel_antidomain_kleene_algebra.ads_d_def
-  by(auto simp: bb_real_arith p2r_def rel_antidomain_kleene_algebra.fbox_def rel_ad_def)
-
-subsubsection{* Circular motion with invariants *}
-
-lemma two_eq_zero: "(2::2) = 0" by simp
-
-lemma [simp]:"i \<noteq> (0::2) \<Longrightarrow> i = 1" using exhaust_2 by fastforce
-
-lemma UNIV_2:"(UNIV::2 set) = {0, 1}"
-  apply safe using exhaust_2 two_eq_zero by auto
-
-lemma sum_axis_UNIV_2[simp]:"(\<Sum>j\<in>(UNIV::2 set). axis i r $ j \<cdot> f j) = r \<cdot> (f::2 \<Rightarrow> real) i"
-  unfolding axis_def UNIV_2 by simp
-
-abbreviation "Circ \<equiv> (\<chi> i. if i= (0::2) then axis (1::2) (- 1::real) else axis 0 1)"
-
-abbreviation "flow_for_Circ t s \<equiv> (\<chi> i. if i= (0::2) then 
-s$0 \<cdot> cos t - s$1 \<cdot> sin t else s$0 \<cdot> sin t + s$1 \<cdot> cos t)"
-
-lemma entries_Circ:"entries Circ = {0, - 1, 1}"
-  apply (simp_all add: axis_def, safe)
-  subgoal by(rule_tac x="0" in exI, simp)+
-  subgoal by(rule_tac x="0" in exI, simp)+
-  by(rule_tac x="1" in exI, simp)+
-
-lemma Circ_is_picard_ivp:"0 \<le> t \<Longrightarrow> t < 1/4 \<Longrightarrow> 
-picard_ivp (\<lambda> t s. Circ *v s) {0..t} UNIV ((real CARD(2))\<^sup>2 \<cdot> maxAbs Circ) 0"
-  apply(rule picard_ivp_linear_system)
-  unfolding entries_Circ by auto
-
-lemma flow_for_Circ_solves_Circ: "((\<lambda> \<tau>. flow_for_Circ \<tau> s) solves_ode (\<lambda>t s.  Circ *v s)) {0..t} UNIV"
-  apply (rule solves_vec_lambda, clarsimp)
-  subgoal for i apply(cases "i=0")
-     apply(simp_all add: matrix_vector_mult_def)
-    unfolding solves_ode_def has_vderiv_on_def has_vector_derivative_def apply auto
-    subgoal for x
-      apply(rule_tac f'1="\<lambda>t. - s$0 \<cdot> (t \<cdot> sin x)" and g'1="\<lambda>t. s$1 \<cdot> (t \<cdot> cos x)"in derivative_eq_intros(11))
-      apply(rule derivative_eq_intros(6)[of cos "(\<lambda>xa. - (xa \<cdot> sin x))"])
-       apply(rule_tac Db1="1" in derivative_eq_intros(58))
-          apply(rule ssubst[of "(\<cdot>) 1" id], force, simp, force, force)
-       apply(rule derivative_eq_intros(6)[of sin "(\<lambda>xa. (xa \<cdot> cos x))"])
-        apply(rule_tac Db1="1" in derivative_eq_intros(55))
-         apply(rule ssubst[of "(\<cdot>) 1" id], force, simp, force, force)
-      by (simp add: Groups.mult_ac(3) Rings.ring_distribs(4))
-    subgoal for x
-      apply(rule_tac f'1="\<lambda>t. s$0 \<cdot> (t \<cdot> cos x)" and g'1="\<lambda>t. - s$1 \<cdot> (t \<cdot> sin x)"in derivative_eq_intros(8))
-      apply(rule derivative_eq_intros(6)[of sin "(\<lambda>xa. xa \<cdot> cos x)"])
-       apply(rule_tac Db1="1" in derivative_eq_intros(55))
-          apply(rule ssubst[of "(\<cdot>) 1" id], force, simp, force, force)
-       apply(rule derivative_eq_intros(6)[of cos "(\<lambda>xa. - (xa \<cdot> sin x))"])
-        apply(rule_tac Db1="1" in derivative_eq_intros(58))
-         apply(rule ssubst[of "(\<cdot>) 1" id], force, simp, force, force)
-      by (simp add: Groups.mult_ac(3) Rings.ring_distribs(4))
-    done
-  done
-
-corollary flow_for_Circ_DS:
-  assumes "0 \<le> t" and "t < 1/4"
-  shows " wp {[x\<acute>=\<lambda> t s. Circ *v s]{0..t} UNIV @ 0 & G} \<lceil>Q\<rceil> = 
-    \<lceil>\<lambda> x. \<forall> \<tau> \<in> {0..t}. (\<forall>r\<in>{0--\<tau>}. G (flow_for_Circ r x)) \<longrightarrow> Q (flow_for_Circ \<tau> x)\<rceil>"
-  apply(subst picard_ivp.wp_g_orbit[of "\<lambda>t s. Circ *v s" _ _ "((real CARD(2))\<^sup>2 \<cdot> maxAbs Circ)" _ 
-"(\<lambda> t x. flow_for_Circ t x)"])
-  using Circ_is_picard_ivp and assms apply blast apply(clarify, rule conjI)
-  using flow_for_Circ_solves_Circ apply blast
-   apply(simp add: vec_eq_iff) using exhaust_2 two_eq_zero apply force 
-  by simp
-
-lemma circular_motion:
-  assumes "0 \<le> t" and "t < 1/4" and "(R::real) > 0"
-  shows"\<lceil>\<lambda>s. R\<^sup>2 = (s $ (0::2))\<^sup>2 + (s $ 1)\<^sup>2\<rceil> \<subseteq> wp 
-  {[x\<acute>=\<lambda>t s. Circ *v s]{0..t} UNIV @ 0 & (\<lambda> s. True)}
-  \<lceil>\<lambda>s. R\<^sup>2 = (s $ (0::2))\<^sup>2 + (s $ 1)\<^sup>2\<rceil>"
-  apply(subst flow_for_Circ_DS)
-  using assms by simp_all
-
-lemma circular_motion_invariants:
-  assumes "0 \<le> t" and "t < 1/4" and "(R::real) > 0"
-  shows"\<lceil>\<lambda>s. R\<^sup>2 = (s $ (0::2))\<^sup>2 + (s $ 1)\<^sup>2\<rceil> \<le> wp 
-  {[x\<acute>=\<lambda>t s. Circ *v s]{0..t} UNIV @ 0 & (\<lambda> s. s $ 0 \<ge> 0)}
-  \<lceil>\<lambda>s. R\<^sup>2 = (s $ (0::2))\<^sup>2 + (s $ 1)\<^sup>2\<rceil>"
-  using assms(1) apply(rule_tac C="\<lambda>s. R\<^sup>2 = (s $ (0::2))\<^sup>2 + (s $ 1)\<^sup>2" in dCut_interval, simp)
-   apply(subgoal_tac "(\<lambda>s. (s $ (0::2))\<^sup>2 + (s $ 1)\<^sup>2 - R\<^sup>2 = 0) = (\<lambda>s. R\<^sup>2 = (s $ (0::2))\<^sup>2 + (s $ 1)\<^sup>2)")
-    apply(rule ssubst[of "(\<lambda>s. R\<^sup>2 = (s $ (0::2))\<^sup>2 + (s $ 1)\<^sup>2)" "\<lambda>s. (s $ (0::2))\<^sup>2 + (s $ 1)\<^sup>2 - R\<^sup>2 = 0"], simp) 
-    apply(rule_tac \<theta>="\<lambda>s. (s $ 0)\<^sup>2 + (s $ 1)\<^sup>2 - R\<^sup>2" and \<nu>="\<lambda>s. 0" in dInvariant_eq_0)
-  subgoal apply clarify
-    apply(frule_tac i="0" in solves_vec_nth, drule_tac i="1" in solves_vec_nth)
-    apply(unfold solves_ode_def has_vderiv_on_def has_vector_derivative_def, clarsimp)
-    apply(erule_tac x="r" in ballE, simp_all add: matrix_vector_mult_def)+
-    apply(rule_tac f'1="\<lambda>t. 0" and g'1="\<lambda>t. 0" in derivative_eq_intros(11))
-      apply(rule_tac f'1="\<lambda>t. - 2 \<cdot> (x r $ 0) \<cdot> (t \<cdot> x r $ 1)" and 
-        g'1="\<lambda>t. 2 \<cdot> (x r $ 1) \<cdot> t \<cdot> x r $ 0" in derivative_eq_intros(8))
-        apply(rule_tac f'1="\<lambda>t. - (t \<cdot> x r $ 1)" in derivative_eq_intros(15))
-         apply (simp add: has_derivative_within_subset, force)
-       apply(rule_tac f'1="\<lambda>t. (t \<cdot> x r $ 0)" in derivative_eq_intros(15))
-        apply (simp add: has_derivative_within_subset) by auto
-  apply(simp, simp, simp, simp add: \<open>0 \<le> t\<close>) apply auto[1]
-  by(rule dWeakening, simp)
+  apply(simp add: rel_antidomain_kleene_algebra.fbox_def)
+  unfolding rel_antidomain_kleene_algebra.cond_def p2r_def
+  by(auto simp: bb_real_arith rel_ad_def rel_antidomain_kleene_algebra.ads_d_def)
 
 end
